working through

src/Pipit.Exp.Causality.fst
@@ -2,123 +2,92 @@
 module Pipit.Exp.Causality
 
 open Pipit.Exp.Base
-open Pipit.Exp.Subst
-open Pipit.Exp.Bigstep
+open Pipit.Exp.Binding
+// open Pipit.Exp.Bigstep
 
 module C = Pipit.Context
 
-(*
 (* Causality: does expression `e` have a dependency on the most-recent value of expression `e'`?
     *)
-let rec direct_dependency (e e': exp) : bool =
-  if e = e' then true
-  else
+let rec direct_dependency (e: exp 'c 'a) (i: C.index { C.has_index 'c i }) : Tot bool (decreases e) =
   match e with
   | XVal _ -> false
-  | XVar x' -> false
-  | XPrim2 _ e1 e2 -> direct_dependency e1 e' || direct_dependency e2 e'
-  | XIte ep et ef -> direct_dependency ep e' || direct_dependency et e' || direct_dependency ef e'
-  | XThen e1 e2 -> direct_dependency e1 e' || direct_dependency e2 e'
-  | XPre _ -> false
-  | XMu e1 -> direct_dependency e1 (lift e' 0)
-  | XLet e1 e2 -> direct_dependency e1 e' || direct_dependency e2 (lift e' 0)
+  | XVar _ -> false
+  | XBVar i' -> i = i'
+  | XApp e1 e2 -> direct_dependency e1 i || direct_dependency e2 i
+  | XFby _ _ -> false
+  | XThen e1 e2 -> direct_dependency e1 i || direct_dependency e2 i
+  | XMu _ e1 -> direct_dependency e1 (i + 1)
+  | XLet b e1 e2 -> direct_dependency e1 i || direct_dependency e2 (i + 1)
+  | XCheck name e1 e2 -> direct_dependency e1 i || direct_dependency e2 i
 
-let rec causal (e: exp): bool =
+let rec causal (e: exp 'c 'a): Tot bool (decreases e) =
   match e with
   | XVal _ -> true
-  | XVar x' -> true
-  | XPrim2 _ e1 e2 -> causal e1 && causal e2
-  | XIte ep e1 e2 -> causal ep && causal e1 && causal e2
+  | XVar _ -> true
+  | XBVar _ -> true
+  | XApp e1 e2 -> causal e1 && causal e2
+  | XFby _ e1 -> causal e1
   | XThen e1 e2 -> causal e1 && causal e2
-  | XPre e1 -> causal e1
-  | XMu e1 -> causal e1 && not (direct_dependency e1 (XVar 0))
-  | XLet e1 e2 -> causal e1 && causal e2
+  | XMu _ e1 -> causal e1 && not (direct_dependency e1 0)
+  | XLet b e1 e2 -> causal e1 && causal e2
+  | XCheck _ e1 e2 -> causal e1 && causal e2
 
-let rec causal_up_to_depth (e: exp) (n: nat): bool =
-  if n = 0 then true
-  else
-    match e with
-    | XVal _ -> true
-    | XVar x' -> true
-    | XPrim2 _ e1 e2 -> causal_up_to_depth e1 n && causal_up_to_depth e2 n
-    | XIte ep e1 e2 -> causal_up_to_depth ep n && causal_up_to_depth e1 n && causal_up_to_depth e2 n
-    | XThen e1 e2 -> causal_up_to_depth e1 n && causal_up_to_depth e2 n
-    | XPre e1 -> causal_up_to_depth e1 (n - 1)
-    | XMu e1 -> causal_up_to_depth e1 n && not (direct_dependency e1 (XVar 0))
-    | XLet e1 e2 -> causal_up_to_depth e1 n && causal_up_to_depth e2 n
+let rec direct_dependency_lift (e: exp 'c 'a) (i: C.index { C.has_index 'c i }) (i': C.index { i' <= List.Tot.length 'c }) (t: Type):
+    Lemma (ensures direct_dependency e i == direct_dependency (lift1' e i' t) (i + 1)) (decreases e) =
+  admit ()
 
-let rec lift_inj (e e': exp) (x: var):
-  Lemma (ensures (e = e') == (lift e x = lift e' x)) =
-  match e, e' with
-  | XVal _, XVal _ -> ()
-  | XVar _, XVar _ -> ()
-  | XPrim2 p e1 e2, XPrim2 _ e1' e2' ->
-    lift_inj e1 e1' x; lift_inj e2 e2' x
-  | XIte ep e1 e2, XIte ep' e1' e2' ->
-    lift_inj ep ep' x; lift_inj e1 e1' x; lift_inj e2 e2' x
-  | XPre e1, XPre e1' -> lift_inj e1 e1' x
-  | XThen e1 e2, XThen e1' e2' ->
-    lift_inj e1 e1' x; lift_inj e2 e2' x
-  | XMu e1, XMu e1' -> lift_inj e1 e1' (x + 1)
-  | XLet e1 e2, XLet e1' e2' ->
-    lift_inj e1 e1' x;
-    lift_inj e2 e2' (x + 1)
-  | _, _ -> ()
+  // match e with
+  // | XVal _ -> ()
+  // | XVar _ -> ()
+  // | XPrim2 p e1 e2 ->
+  //   direct_dependency_lift e1 e' x;
+  //   direct_dependency_lift e2 e' x
+  // | XIte ep e1 e2 ->
+  //   direct_dependency_lift ep e' x;
+  //   direct_dependency_lift e1 e' x;
+  //   direct_dependency_lift e2 e' x
+  // | XPre _ -> ()
+  // | XThen e1 e2 ->
+  //   direct_dependency_lift e1 e' x;
+  //   direct_dependency_lift e2 e' x
+  // | XMu e1 ->
+  //   direct_dependency_lift e1 (lift e' 0) (x + 1);
+  //   lift_lift_commute e' x 0
+  // | XLet e1 e2 ->
+  //   direct_dependency_lift e1 e' x;
+  //   direct_dependency_lift e2 (lift e' 0) (x + 1);
+  //   lift_lift_commute e' x 0
 
-let rec direct_dependency_lift (e e': exp) (x: var):
-    Lemma (ensures direct_dependency e e' == direct_dependency (lift e x) (lift e' x)) (decreases e) =
-  lift_inj e e' x;
-  match e with
-  | XVal _ -> ()
-  | XVar _ -> ()
-  | XPrim2 p e1 e2 ->
-    direct_dependency_lift e1 e' x;
-    direct_dependency_lift e2 e' x
-  | XIte ep e1 e2 ->
-    direct_dependency_lift ep e' x;
-    direct_dependency_lift e1 e' x;
-    direct_dependency_lift e2 e' x
-  | XPre _ -> ()
-  | XThen e1 e2 ->
-    direct_dependency_lift e1 e' x;
-    direct_dependency_lift e2 e' x
-  | XMu e1 ->
-    direct_dependency_lift e1 (lift e' 0) (x + 1);
-    lift_lift_commute e' x 0
-  | XLet e1 e2 ->
-    direct_dependency_lift e1 e' x;
-    direct_dependency_lift e2 (lift e' 0) (x + 1);
-    lift_lift_commute e' x 0
-
-let rec direct_dependency_not_subst (x: var) (x': var { x' < x })
-  (e: exp { ~ (direct_dependency e (XVar x)) })
-  (p: exp { ~ (direct_dependency p (XVar (x - 1))) }):
-    Lemma (ensures ~ (direct_dependency (subst e x' p) (XVar (x - 1)))) (decreases e) =
-  match e with
-  | XVal _ -> ()
-  | XVar x'' -> ()
-  | XPrim2 prim e1 e2 ->
-    direct_dependency_not_subst x x' e1 p;
-    direct_dependency_not_subst x x' e2 p
-  | XIte ep e1 e2 ->
-    direct_dependency_not_subst x x' ep p;
-    direct_dependency_not_subst x x' e1 p;
-    direct_dependency_not_subst x x' e2 p
-  | XPre _ -> ()
-  | XThen e1 e2 ->
-    direct_dependency_not_subst x x' e1 p;
-    direct_dependency_not_subst x x' e2 p
-  | XMu e1 ->
-    direct_dependency_lift p (XVar (x - 1)) 0;
-    direct_dependency_not_subst (x + 1) (x' + 1) e1 (lift p 0)
-  | XLet e1 e2 ->
-    direct_dependency_lift p (XVar (x - 1)) 0;
-    direct_dependency_not_subst x x' e1 p;
-    direct_dependency_not_subst (x + 1) (x' + 1) e2 (lift p 0)
-*)
+let rec direct_dependency_not_subst (i: C.index { C.has_index 'c i }) (i': C.index { i' < i })
+  (e: exp 'c 'a { ~ (direct_dependency e i) })
+  (p: exp (C.drop1 'c i') (C.get_index 'c i') { ~ (direct_dependency p (i - 1)) }):
+    Lemma (ensures ~ (direct_dependency (subst1' e i' p) (i - 1))) (decreases e) =
+  admit ()
+  // match e with
+  // | XVal _ -> ()
+  // | XVar x'' -> ()
+  // | XPrim2 prim e1 e2 ->
+  //   direct_dependency_not_subst x x' e1 p;
+  //   direct_dependency_not_subst x x' e2 p
+  // | XIte ep e1 e2 ->
+  //   direct_dependency_not_subst x x' ep p;
+  //   direct_dependency_not_subst x x' e1 p;
+  //   direct_dependency_not_subst x x' e2 p
+  // | XPre _ -> ()
+  // | XThen e1 e2 ->
+  //   direct_dependency_not_subst x x' e1 p;
+  //   direct_dependency_not_subst x x' e2 p
+  // | XMu e1 ->
+  //   direct_dependency_lift p (XVar (x - 1)) 0;
+  //   direct_dependency_not_subst (x + 1) (x' + 1) e1 (lift p 0)
+  // | XLet e1 e2 ->
+  //   direct_dependency_lift p (XVar (x - 1)) 0;
+  //   direct_dependency_not_subst x x' e1 p;
+  //   direct_dependency_not_subst (x + 1) (x' + 1) e2 (lift p 0)
 
 (* Shelve: proofs about causality, will need to be restated on single-element semantics *)
-(*
+
 let rec direct_dependency_not_subst2 (x: var) (x': var { x < x' }) (e p: exp):
     Lemma
       (requires not (direct_dependency (subst e x' p) (XVar x)))
@@ -139,26 +108,6 @@ let rec direct_dependency_not_subst2 (x: var) (x': var { x < x' }) (e p: exp):
   | XLet e1 e2 ->
     direct_dependency_not_subst2 x x' e1 p;
     direct_dependency_not_subst2 (x + 1) (x' + 1) e2 (lift p 0)
-
-let rec causal_up_to_depth_lift (e: exp) (x: var) (n: nat):
-    Lemma (ensures causal_up_to_depth e n == causal_up_to_depth (lift e x) n) =
-  match e with
-  | XVal _ -> ()
-  | XVar _ -> ()
-  | XPrim2 p e1 e2 ->
-    causal_up_to_depth_lift e1 x n;
-    causal_up_to_depth_lift e2 x n
-  | XPre e1 -> if n > 0 then causal_up_to_depth_lift e1 x (n - 1)
-  | XThen e1 e2 ->
-    causal_up_to_depth_lift e1 x n;
-    causal_up_to_depth_lift e2 x n
-  | XMu e1 ->
-    causal_up_to_depth_lift e1 (x + 1) n;
-    lift_lift_commute e1 (x + 1) 0;
-    direct_dependency_lift e1 (XVar 0) (x + 1)
-  | XLet e1 e2 ->
-    causal_up_to_depth_lift e1 x n;
-    causal_up_to_depth_lift e2 (x + 1) n
 
 
 let rec bigstep_no_dep_no_difference (#outer #inner1 #inner2: nat) (e: exp { ~ (direct_dependency e (XVar inner1)) })
@@ -237,85 +186,32 @@ let rec bigstep_no_dep_no_difference (#outer #inner1 #inner2: nat) (e: exp { ~ (
 //     Lemma (ensures causal e) (decreases hBS) =
 //
 
-let rec causal_up_to_subst1 (e e': exp) (x: var) (n: nat):
-  Lemma (requires causal_up_to_depth (subst e x e') n)
-        (ensures causal_up_to_depth e n) =
-  if n = 0 then ()
-  else
-    match e with
-    | XPrim2 _ e1 e2 -> causal_up_to_subst1 e1 e' x n; causal_up_to_subst1 e2 e' x n
-    | XMu e1 ->
-      causal_up_to_subst1 e1 (lift e' 0) (x + 1) n;
-      direct_dependency_not_subst2 0 (x + 1) e1 (lift e' 0);
-      ()
-    | XPre e1 -> causal_up_to_subst1 e1 e' x (n - 1)
-    | XThen e1 e2 -> causal_up_to_subst1 e1 e' x n; causal_up_to_subst1 e2 e' x n
-    | XLet e1 e2 -> causal_up_to_subst1 e1 e' x n; causal_up_to_subst1 e2 (lift e' 0) (x + 1) n
-    | _ -> ()
-
+// XXX: cannot state this on direct_dependency with var...
+// but can state:
 let rec direct_dep_XVar__direct_dep_subst (e e': exp) (x: var):
-  Lemma (requires direct_dependency e (XVar x))
-        (ensures direct_dependency (subst e x e') e') =
-  match e with
-  | XPrim2 _ e1 e2 ->
-    if direct_dependency e1 (XVar x)
-    then direct_dep_XVar__direct_dep_subst e1 e' x
-    else direct_dep_XVar__direct_dep_subst e2 e' x
-  | XMu e1 ->
-    direct_dep_XVar__direct_dep_subst e1 (lift e' 0) (x + 1)
-  | XThen e1 e2 ->
-    if direct_dependency e1 (XVar x)
-    then direct_dep_XVar__direct_dep_subst e1 e' x
-    else direct_dep_XVar__direct_dep_subst e2 e' x
-  | XLet e1 e2 ->
-    if direct_dependency e1 (XVar x)
-    then direct_dep_XVar__direct_dep_subst e1 e' x
-    else direct_dep_XVar__direct_dep_subst e2 (lift e' 0) (x + 1)
-  | _ -> ()
-
-let rec direct_dep_acausal__acausal (e e': exp) (n: nat):
-  Lemma (requires direct_dependency e e' /\ not (causal_up_to_depth e' n))
-        (ensures not (causal_up_to_depth e n)) =
-  if e = e' then ()
-  else
-  match e with
-  | XPrim2 p e1 e2 ->
-    if direct_dependency e1 e'
-    then direct_dep_acausal__acausal e1 e' n
-    else direct_dep_acausal__acausal e2 e' n
-  | XMu e1 ->
-    assert (direct_dependency e1 (lift e' 0));
-    causal_up_to_depth_lift e' 0 n;
-    direct_dep_acausal__acausal e1 (lift e' 0) n;
-    ()
-  | XThen e1 e2 ->
-    if direct_dependency e1 e'
-    then direct_dep_acausal__acausal e1 e' n
-    else direct_dep_acausal__acausal e2 e' n
-  | XLet e1 e2 ->
-    causal_up_to_depth_lift e' 0 n;
-    if direct_dependency e1 e'
-    then direct_dep_acausal__acausal e1 e' n
-    else direct_dep_acausal__acausal e2 (lift e' 0) n
-  | _ -> ()
-
-let causal_up_to_depth_subst_XMu (e: exp) (n: nat):
-  Lemma (requires causal_up_to_depth (subst e 0 (XMu e)) n)
-        (ensures causal_up_to_depth (XMu e) n) =
-  if n = 0
-  then ()
-  else begin
-    if direct_dependency e (XVar 0)
-    then
-    begin
-      assert (not (causal_up_to_depth (XMu e) n));
-      direct_dep_XVar__direct_dep_subst e (XMu e) 0;
-      direct_dep_acausal__acausal (subst e 0 (XMu e)) (XMu e) n;
-      ()
-    end
-    else
-      causal_up_to_subst1 e (XMu e) 0 n
-  end
+  Lemma (requires direct_dependency e x /\ direct_dependency e' x')
+        (ensures direct_dependency (subst e x e') x') =
+  admit ()
+//
+// let rec direct_dep_XVar__direct_dep_subst (e e': exp) (x: var):
+//   Lemma (requires direct_dependency e (XVar x))
+//         (ensures direct_dependency (subst e x e') e') =
+//   match e with
+//   | XPrim2 _ e1 e2 ->
+//     if direct_dependency e1 (XVar x)
+//     then direct_dep_XVar__direct_dep_subst e1 e' x
+//     else direct_dep_XVar__direct_dep_subst e2 e' x
+//   | XMu e1 ->
+//     direct_dep_XVar__direct_dep_subst e1 (lift e' 0) (x + 1)
+//   | XThen e1 e2 ->
+//     if direct_dependency e1 (XVar x)
+//     then direct_dep_XVar__direct_dep_subst e1 e' x
+//     else direct_dep_XVar__direct_dep_subst e2 e' x
+//   | XLet e1 e2 ->
+//     if direct_dependency e1 (XVar x)
+//     then direct_dep_XVar__direct_dep_subst e1 e' x
+//     else direct_dep_XVar__direct_dep_subst e2 (lift e' 0) (x + 1)
+//   | _ -> ()
 
 let causal_subst__causal_XMu (e: exp) (n: nat):
   Lemma (requires causal (XMu e))
@@ -324,39 +220,12 @@ let causal_subst__causal_XMu (e: exp) (n: nat):
   admit ()
 
 
-let rec bigstep_means_causal_up_to_depth (#outer #inner: nat) (e: exp)
-  (streams: C.table outer inner)
-  (vs: C.vector value outer)
-  (hBS: bigstep streams e vs):
-    Lemma (ensures causal_up_to_depth e outer) (decreases hBS) =
-  match hBS with
-  | BSVal _ _ -> ()
-  | BSVar _ x' -> ()
-  | BSPrim2 _ p e1' e2' vs1 vs2 hBS1 hBS2 ->
-    let XPrim2 _ e1 e2 = e in
-    bigstep_means_causal_up_to_depth e1 streams vs1 hBS1;
-    bigstep_means_causal_up_to_depth e2 streams vs2 hBS2
-  | BSMu _ e1' vs1 hBS1 ->
-    let XMu e1 = e in
-    bigstep_means_causal_up_to_depth (subst e1 0 (XMu e1)) streams vs1 hBS1;
-    causal_up_to_depth_subst_XMu e1 outer
-  | BSPre _ streams' e1 vs1 hBS1 ->
-    bigstep_means_causal_up_to_depth e1 streams' vs1 hBS1
-  | BSPre0 _ -> ()
-  | BSThen _ e1 e2 vs1 vs2 hBS1 hBS2 ->
-    bigstep_means_causal_up_to_depth e1 streams vs1 hBS1;
-    bigstep_means_causal_up_to_depth e2 streams vs2 hBS2
-  | BSLet _ e1' e2' vs2 hBS2 ->
-  // TODO BSLet
-    admit ()
-
-
 let bigstep_recursive_XMu (#outer #inner: nat) (e: exp)
   (streams: C.table (outer + 1) inner)
   (vs: C.vector value outer) (v v': value)
   (hBSmu: bigstep streams (XMu e) (v :: vs)):
     bigstep (C.table_map_append (C.table_of_values (v' :: vs)) streams) e (v :: vs) =
-    bigstep_means_causal_up_to_depth _ _ _ hBSmu;
+    // bigstep_means_causal_up_to_depth _ _ _ hBSmu;
     let hBS' = bigstep_substitute_XMu e streams _ hBSmu in
     C.table_map_append_empty1 (C.table_map_append (C.table_of_values (v :: vs)) streams);
     C.table_map_append_empty1 (C.table_map_append (C.table_of_values (v' :: vs)) streams);
@@ -422,4 +291,3 @@ let bigstep_monotone_inv (#outer #inner: nat)
     Tot (bigstep streams e (bigstep_monotone_inv_next hBS :: vs)) =
   let (| v', hBS' |) = bigstep_monotone_inv' hBS in hBS'
 
-*)
